\paragraph{组合公式}
\begin{itemize}
\item
fibonacci\\
$f_0=0, f_1=1$\\
$f_{n+2}f_n-f_{n+1}^2=(-1)^{n+1}$\\
$f_{-n}=(-1)^{n-1}f_n$\\
$f_{n+k}=f_kf_{n+1}+f_{k-1}f_n$\\
$gcd(f_m, f_n)=f_{gcd(m, n)}$\\
$f_m|f_n^2\Leftrightarrow nf_n|m$\\

\item
  $\sum_{k=1}^{n}(2k-1)^2 = \frac{n(4n^2-1)}{3}	$
\item
  $\sum_{k=1}^{n}k^3 = (\frac{n(n+1)}{2})^2	$
\item
  $\sum_{k=1}^{n}(2k-1)^3 = n^2(2n^2-1)	$
\item
  $\sum_{k=1}^{n}k^4 = \frac{n(n+1)(2n+1)(3n^2+3n-1)}{30}  $
\item
  $\sum_{k=1}^{n}k^5 = \frac{n^2(n+1)^2(2n^2+2n-1)}{12}	$
\item
  $\sum_{k=1}^{n}k(k+1) = \frac{n(n+1)(n+2)}{3}	$
\item
  $\sum_{k=1}^{n}k(k+1)(k+2) = \frac{n(n+1)(n+2)(n+3)}{4} $
\item
  $\sum_{k=1}^{n}k(k+1)(k+2)(k+3) = \frac{n(n+1)(n+2)(n+3)(n+4)}{5} $
\item
  $\mbox{错排：}D_n = n!(1-\frac{1}{1!}+\frac{1}{2!}-\frac{1}{3!}+\ldots+\frac{(-1)^n}{n!}) = (n-1)(D_{n-2}-D_{n-1})$
\end{itemize}

